\label{ExercisesforAppDerivatives}
In Exercises \ref{diffquotexerfirsta} - \ref{diffquotexerlasta}, find the limit of the following difference quotients.

\begin{multicols}{2}

\begin{itemize}

\item  $\ds{\lim_{h \rightarrow 0} \dfrac{f(2+h) - f(2)}{h}}$

\item  $\ds{\lim_{h \rightarrow 0} \dfrac{f(x+h) - f(x)}{h}}$

\end{itemize}

\end{multicols}


\begin{multicols}{2}

\begin{enumerate}


\item $f(x) = 2x - 5$ \label{diffquotexerfirsta}
\item $f(x) = -3x + 5$

\setcounter{HW}{\value{enumi}}
\end{enumerate}
\end{multicols}

\begin{multicols}{2}
\begin{enumerate}
\setcounter{enumi}{\value{HW}}

\item $f(x) = 6$
\item $f(x) = 3x^2 - x$

\setcounter{HW}{\value{enumi}}
\end{enumerate}
\end{multicols}

\begin{multicols}{2}
\begin{enumerate}
\setcounter{enumi}{\value{HW}}

\item $f(x) = -x^2 + 2x - 1$
\item\label{diffquotexerlasta}  $f(x) = 4x^2$ 

\setcounter{HW}{\value{enumi}}
\end{enumerate}
\end{multicols}


In Exercises \ref{tangentlinepolyfirst} - \ref{tangentlinepolylast}, find:


\begin{itemize}

\item  $f'(2)  = \ds{\lim_{h \rightarrow 0} \dfrac{f(2+h) - f(2)}{h}}$

\item  The equation of the tangent line at $(2, f(2))$.  Check your answer graphically.

\item  $f'(x) = \ds{\lim_{h \rightarrow 0} \dfrac{f(x+h) - f(x)}{h}}$

\item  The equation of the tangent line at $(0,f(0))$.  Check your answer graphically.
 
\end{itemize}



\begin{multicols}{2}
\begin{enumerate}
\setcounter{enumi}{\value{HW}}

\item\label{tangentlinepolyfirst}  $f(x) = x-x^2$ 
\item\label{tangentlinepolylast} $f(x) = x^{3} + 1$

\setcounter{HW}{\value{enumi}}
\end{enumerate}
\end{multicols}




\begin{enumerate}
\setcounter{enumi}{\value{HW}}

\item  Find $f'(x) = \ds{\lim_{h \rightarrow 0} \dfrac{f(x+h) - f(x)}{h}}$  for $f(x) = mx + b\;$ where $m \neq 0$

\item \begin{enumerate}  \item Find $f'(x) = \ds{\lim_{h \rightarrow 0} \dfrac{f(x+h) - f(x)}{h}}$   for  $f(x) = ax^{2} + bx + c\;$ where $a \neq 0$.

\item  Solve $f'(x) = 0$ for $x$.  Does this look familiar?  Explain.

\end{enumerate}

\setcounter{HW}{\value{enumi}}
\end{enumerate}





In Exercises \ref{diffquotexerfirstb} - \ref{diffquotexerlastb}, find the limit of the following difference quotients:

\begin{multicols}{2}

\begin{itemize}

\item  $\ds{\lim_{\Delta x \rightarrow 0} \dfrac{f(-1+\Delta x) - f(-1)}{\Delta x}}$

\item  $\ds{\lim_{\Delta x \rightarrow 0} \dfrac{f(x+\Delta x) - f(x)}{\Delta x}}$

\end{itemize}

\end{multicols}

\begin{multicols}{2}
\begin{enumerate}
\setcounter{enumi}{\value{HW}}

\item $f(x) = \dfrac{2}{x}$  \label{diffquotexerfirstb}
\item $f(x) = \dfrac{3}{1-x}$

\setcounter{HW}{\value{enumi}}
\end{enumerate}
\end{multicols}

\begin{multicols}{2}
\begin{enumerate}
\setcounter{enumi}{\value{HW}}

\item  $f(x) = \dfrac{1}{x^2}$
\item\label{diffquotexerlastb}  $f(x) = \dfrac{2}{x+5}$

\setcounter{HW}{\value{enumi}}
\end{enumerate}
\end{multicols}

In Exercises \ref{rationaltangentfirst} - \ref{rationaltangentlast}, find the limit of the following:



\begin{itemize}

\item  $f'(-1) = \ds{\lim_{\Delta x \rightarrow 0} \dfrac{f(-1+\Delta x) - f(-1)}{\Delta x}}$

\item The equation of the tangent line at $(-1, f(-1))$.

\item  $f'(x) = \ds{\lim_{\Delta x \rightarrow 0} \dfrac{f(x+\Delta x) - f(x)}{\Delta x}}$

\item  The equation of the tangent line at $(0,f(0))$.

\end{itemize}

\begin{multicols}{2}
\begin{enumerate}

\setcounter{enumi}{\value{HW}}

\item\label{rationaltangentfirst} $f(x) = \dfrac{1}{4x-3}$ 
\item $f(x) = \dfrac{3x}{x+2}$ 

\setcounter{HW}{\value{enumi}}
\end{enumerate}
\end{multicols}

\begin{multicols}{2}
\begin{enumerate}
\setcounter{enumi}{\value{HW}}

\item $f(x) = \dfrac{x}{x - 9}$
\item\label{rationaltangentlast} $f(x) = \dfrac{x^2}{2x+1}$ 

\setcounter{HW}{\value{enumi}}
\end{enumerate}
\end{multicols}

In Exercises \ref{diffquotexerfirstc} - \ref{diffquotexerlastc},  find the limit of the following difference quotients:

\begin{multicols}{2}

\begin{itemize}

\item  $\ds{\lim_{\Delta t \rightarrow 0} \dfrac{g(\Delta t) - g(0)}{\Delta t}}$

\item  $\ds{\lim_{\Delta t \rightarrow 0} \dfrac{g(t+\Delta t) - g(t)}{\Delta t}}$

\end{itemize}

\end{multicols}


\begin{multicols}{2}
\begin{enumerate}
\setcounter{enumi}{\value{HW}}

\item  $g(t) = \sqrt{9-t}$  \label{diffquotexerfirstc}
\item  $g(t) = \sqrt{2t+1}$   \label{diffquotexerlastc}


\setcounter{HW}{\value{enumi}}
\end{enumerate}
\end{multicols}

In Exercises \ref{tangentrootfirst} - \ref{tangentrootlast},  find the following:



\begin{itemize}

\item  $g'(0) = \ds{\lim_{\Delta t \rightarrow 0} \dfrac{g(\Delta t) - g(0)}{\Delta t}}$

\item  The equation of the tangent line at $(0, g(0))$.

\item  $g'(t) =  \ds{\lim_{\Delta t \rightarrow 0} \dfrac{g(t+\Delta t) - g(t)}{\Delta t}}$

\item  The equation of the tangent line at $(1, g(1))$.

\end{itemize}




\begin{multicols}{2}
\begin{enumerate}
\setcounter{enumi}{\value{HW}}

\item\label{tangentrootfirst}  $g(t) = \sqrt{-4t+5}$
\item  \label{tangentrootlast} $g(t) = \sqrt{4-t}$


\setcounter{HW}{\value{enumi}}
\end{enumerate}
\end{multicols}



\begin{enumerate}
\setcounter{enumi}{\value{HW}}

\item  For  $g(t) = t \sqrt{t}$:

\begin{enumerate}

\item  Explain why $g'(0) = \ds{\lim_{\Delta t \rightarrow 0} \dfrac{g(\Delta t) - g(0)}{\Delta t}}$ does not exist.

\item Find the \index{derivative from the right}\index{derivative ! from the right} derivative \textbf{from the right} at $t=0$:  $g_{+}'(0) = \ds{\lim_{\Delta t \rightarrow 0^{+}} \dfrac{g(\Delta t) - g(0)}{\Delta t}}$

\item  Find $y = g_{+}'(0) (x-0) + g(0)$ and interpret.

\item Find  $g'(t) =  \ds{\lim_{\Delta t \rightarrow 0} \dfrac{g(t+\Delta t) - g(t)}{\Delta t}}$.  Assume $t>0$.

\end{enumerate}


\item  \begin{enumerate} \item Find  $g'(t) =  \ds{\lim_{\Delta t \rightarrow 0} \dfrac{g(t+\Delta t) - g(t)}{\Delta t}}$ for  $g(t) = \sqrt{at+b}$, $a \neq 0$. 

\smallskip

\item What restrictions do you place on $t$ so your formula is valid?

\end{enumerate}


\setcounter{HW}{\value{enumi}}
\end{enumerate}


\begin{enumerate}
\setcounter{enumi}{\value{HW}}

\item Let  $g(t) = \sqrt[3]{t}$.  

\begin{enumerate}

\item\label{verticaltangentex} Show $g'(0) = \ds{\lim_{\Delta t \rightarrow 0} \dfrac{g(\Delta t) - g(0)}{\Delta t} = \infty}$.  

\smallskip

\textbf{HINT:}  $(a-b)\left(a^2+ab+b^2\right) = a^3 - b^3$ 
        
\smallskip
        
\item  Graph $y = g(t)$ near $t=0$.  Interpret your answer to number \ref{verticaltangentex} graphically.

\smallskip

\item  Find and simplify  $g'(t) =  \ds{\lim_{\Delta t \rightarrow 0} \dfrac{g(t+\Delta t) - g(t)}{\Delta t}}$ assuming $t \neq 0$.

\end{enumerate}

\setcounter{HW}{\value{enumi}}
\end{enumerate}

\newpage

\subsection{Answers}


\begin{enumerate}

\item $\ds{\lim_{h \rightarrow 0} 2 = 2}$, $\ds{\lim_{h \rightarrow 0} 2 = 2}$
\item $\ds{\lim_{h \rightarrow 0} -3 = -3}$, $\ds{\lim_{h \rightarrow 0} -3 = -3}$,

\setcounter{HW}{\value{enumi}}
\end{enumerate}

\begin{enumerate}
\setcounter{enumi}{\value{HW}}

\item $\ds{\lim_{h \rightarrow 0} 0 = 0}$,  $\ds{\lim_{h \rightarrow 0} 0 = 0}$
\item  $\ds{\lim_{h \rightarrow 0} (3h+11)= 11}$,   $\ds{\lim_{h \rightarrow 0} (6x+3h-1)= 6x-1}$

\setcounter{HW}{\value{enumi}}
\end{enumerate}

\begin{enumerate}
\setcounter{enumi}{\value{HW}}

\item    $\ds{\lim_{h \rightarrow 0} (-h-2) = -2}$,   $\ds{\lim_{h \rightarrow 0} (-2x-h+2) = -2x+2}$   
\item   $\ds{\lim_{h \rightarrow 0} (4h+16) = 16}$,   $\ds{\lim_{h \rightarrow 0} (8x+4h) = 8x}$ 

\setcounter{HW}{\value{enumi}}
\end{enumerate}

\begin{enumerate}
\setcounter{enumi}{\value{HW}}

\item \begin{itemize}  \item $f'(2) = \ds{\lim_{h \rightarrow 0} (-h-3) = -3}$

\smallskip

\item  $y = f'(2)(x-2) + f(2) = (-3)(x-2)+(-2)$ so $y  = -3x+4$.

\smallskip

\item   $f'(x) =  \ds{\lim_{h \rightarrow 0} (-2x-h+1) = -2x+1}$ 

\smallskip

\item  $y = f'(0)(x-0) + f(0) = (1)(x-0) + 0$ so $y = x$.

\smallskip

\end{itemize}

\item \begin{itemize}

\item $f'(2) = \ds{\lim_{h \rightarrow 0} \left( h^2+6h+12 \right) = 12}$

\smallskip

\item  $y = f'(2)(x-2) + f(2) = 12(x-2)+ 9$ so $y = 12x - 15$.

\smallskip

\item  $f'(x) = \ds{\lim_{h \rightarrow 0} \left(3x^{2} + 3xh + h^{2} \right) = 3x^{2}}$ 

\smallskip

\item $y = f'(0)(x-0)+f(0) = 0(x-0)+1$ so $y = 1$.

\smallskip

\end{itemize} 

\setcounter{HW}{\value{enumi}}
\end{enumerate}

\begin{enumerate}
\setcounter{enumi}{\value{HW}}

\item  $f'(x) = \ds{\lim_{h \rightarrow 0} m= m}$.

\item  \begin{itemize} \item  $f'(x) = \ds{\lim_{h \rightarrow 0} (2ax + ah + b) = 2ax + b}$.

\smallskip

\item  Solving $f'(x) = 2ax + b = 0$ for $x$ gives $x = -\frac{b}{2a}$ which is the formula for the $x$-coordinate of the vertex of the parabola $y = f(x)$.  If we zoom in near the the vertex of a parabola, the graph becomes locally flat so it makes sense the slope of the tangent line,  $f'(x) = 0$ there. 

\end{itemize} 

\setcounter{HW}{\value{enumi}}
\end{enumerate}

\begin{enumerate}
\setcounter{enumi}{\value{HW}}

\item  $\ds{ \lim_{\Delta x \rightarrow 0} \dfrac{2}{\Delta x-1} = -2}$,   $\ds{ \lim_{\Delta x \rightarrow 0} \dfrac{-2}{x(x+\Delta x)} = - \dfrac{2}{x^2}}$
 
\item  $\ds{ \lim_{\Delta x \rightarrow 0} \dfrac{-3}{2(\Delta x - 2)} = \dfrac{3}{4}}$,   $\ds{ \lim_{\Delta x \rightarrow 0} \dfrac{3}{(x+\Delta x-1)(x-1)} =  \dfrac{3}{(x-1)^2}}$  

\setcounter{HW}{\value{enumi}}
\end{enumerate}

\begin{enumerate}
\setcounter{enumi}{\value{HW}}

\item   $\ds{ \lim_{\Delta x \rightarrow 0} \dfrac{2-\Delta x}{(\Delta x - 1)^2} =2}$,   $\ds{ \lim_{\Delta x \rightarrow 0}\dfrac{-(2x+\Delta x)}{x^2(x+\Delta x)^2} =  - \dfrac{2}{x^3}}$   

\item    $\ds{ \lim_{\Delta x \rightarrow 0} \dfrac{-1}{2(\Delta x+4)} = - \dfrac{1}{8}}$,   $\ds{ \lim_{\Delta x \rightarrow 0} \dfrac{-2}{(x+5)(x+\Delta x+5)}=  - \dfrac{2}{(x+5)^2}}$    

\setcounter{HW}{\value{enumi}}
\end{enumerate}

\begin{enumerate}
\setcounter{enumi}{\value{HW}}

\item \begin{itemize}

\item  $f'(-1) =\ds{ \lim_{\Delta x \rightarrow 0} \dfrac{4}{7(4 \Delta x - 7)} = - \dfrac{4}{49}}$

\smallskip

\item $y = f'(-1)(x-(-1)) + f(-1) = -\frac{4}{49}(x + 1) + \left(-\frac{1}{7}\right)$ so $y = -\frac{4}{49} \, x - \frac{11}{49}$.   

\smallskip

\item  $f'(x) = \ds{ \lim_{\Delta x \rightarrow 0} \dfrac{-4}{(4x-3)(4x+4\Delta x-3)} =  - \dfrac{4}{(4x-3)^2}}$  

\smallskip

\item $y = f'(0)(x-0)+f(0) = -\frac{4}{9} (x-0) + \left(-\frac{1}{3}\right)$ so $y = -\frac{4}{9} \, x - \frac{1}{3}$.

\smallskip

\end{itemize}
   
\item \begin{itemize}

\item  $f'(-1) = \ds{ \lim_{\Delta x \rightarrow 0} \dfrac{6}{\Delta x + 1}= 6}$

\smallskip

\item $y = f'(-1)(x-(-1)) + f(-1) = 6(x+1) + (-3)$ so $y = 6x+3$.

\smallskip

\item  $f'(x) =\ds{ \lim_{\Delta x \rightarrow 0} \dfrac{6}{(x+2)(x+\Delta x+2)} =   \dfrac{6}{(x+2)^2}}$ 

\smallskip    

\item  $y = f'(0)(x-0) + f(0) = \frac{3}{2} \, (x-0)+0$ so $y = \frac{3}{2} \, x$.


\smallskip


\end{itemize}

 
\setcounter{HW}{\value{enumi}}
\end{enumerate}

\begin{enumerate}
\setcounter{enumi}{\value{HW}}

\item   \begin{itemize}

\item  $f'(-1) = \ds{ \lim_{\Delta x \rightarrow 0} \dfrac{9}{10(\Delta x - 10)} = -\dfrac{9}{100}}$

\smallskip

\item $y = f'(-1)(x-(-1)) + f(-1) = -\frac{9}{100} \, (x+1) + \frac{1}{10}$ so $y = - \frac{9}{100} \, x + \frac{1}{100}$.

\smallskip

\item  $f'(x) =\ds{ \lim_{\Delta x \rightarrow 0} \dfrac{-9}{(x - 9)(x + \Delta x - 9)} =   -\dfrac{9}{(x-9)^2}}$   

\smallskip  

\item  $y = f'(0)(x-0) + f(0) = -\frac{1}{9} \, (x-0)+0$ so $y = -\frac{1}{9} \, x$.

\smallskip

\end{itemize}

\item \begin{itemize}  

\item  $f'(-1) = \ds{ \lim_{\Delta x \rightarrow 0} \dfrac{\Delta x}{2 \Delta x - 1} = 0}$

\smallskip

\item $y = f'(-1)(x-(-1)) + f(-1) = (0) (x+1) + (-1)$ so $y = -1$.

\smallskip

\item  $f'(x) =\ds{ \lim_{\Delta x \rightarrow 0}\dfrac{2x^2+2x\Delta x+2x+\Delta x}{(2x+1)(2x+2\Delta x+1)}=  \dfrac{2x^2+2x}{(2x+1)^2}}$

\smallskip

\item  $y = f'(0)(x-0) + f(0) = (0)(x-0)+0$ so $y = 0$.

\smallskip

\end{itemize}


\setcounter{HW}{\value{enumi}}
\end{enumerate}

\begin{enumerate}
\setcounter{enumi}{\value{HW}}

\item  $\ds{ \lim_{\Delta t \rightarrow 0}\dfrac{-1}{\sqrt{9-\Delta t} +3}  = -\dfrac{1}{6}}$,   $\ds{ \lim_{\Delta t \rightarrow 0} \dfrac{-1}{\sqrt{9-t-\Delta t} + \sqrt{9-t}}=   -\dfrac{1}{2 \sqrt{9-t}}}$   
\item  $\ds{ \lim_{\Delta t \rightarrow 0}\dfrac{2}{\sqrt{2\Delta t+1} + 1}  =1}$,   $\ds{ \lim_{\Delta t \rightarrow 0}\dfrac{2}{\sqrt{2t+2\Delta t+1} + \sqrt{2t+1}}=   \dfrac{2}{2 \sqrt{2t+1}}}$    

\setcounter{HW}{\value{enumi}}
\end{enumerate}

\begin{enumerate}
\setcounter{enumi}{\value{HW}}

\item \begin{itemize}

\item  $g'(0) = \ds{ \lim_{\Delta t \rightarrow 0} \dfrac{-4}{\sqrt{5-4\Delta t} + \sqrt{5}}  = - \dfrac{2}{\sqrt{5}}}$

\smallskip

\item  $y = g'(0) (x - 0) + g(0) =  -\frac{2}{\sqrt{5}} \, (x-0) + \sqrt{5}$ so $y = -\frac{2}{\sqrt{5}} \, x + \sqrt{5}$.

\smallskip

\item  $g'(t) =  \ds{ \lim_{\Delta t \rightarrow 0} \dfrac{-4}{\sqrt{-4t-4\Delta t+5} + \sqrt{-4t+5}} =   -\dfrac{2}{\sqrt{-4t+5}}}$

\smallskip

\item  $y = g'(1)(x-1)+g(1) = (-2)(x-1) + 1$ so $y = -2x+3$.

\smallskip

\end{itemize}

\item   \begin{itemize}

\item  $g'(0) = \ds{ \lim_{\Delta t \rightarrow 0} \dfrac{-1}{\sqrt{4-\Delta t} + 2}  = - \dfrac{1}{4}}$

\smallskip

\item  $y = g'(0) (x - 0) + g(0) =  -\frac{1}{4} \, (x-0) + 2$ so $y = -\frac{1}{4} \, x +2$.

\smallskip

\item  $g'(t) = \ds{ \lim_{\Delta t \rightarrow 0} \dfrac{-1}{\sqrt{4-t-\Delta t} + \sqrt{4-t}} = -\dfrac{1}{2 \sqrt{4-t}} }$  

\smallskip

\item  $y = g'(1)(x-1)+g(1) = -\frac{1}{2 \sqrt{3}} \, (x-1) + \sqrt{3}$ so $y =  -\frac{1}{2 \sqrt{3}}  \, x + \frac{7 \sqrt{3}}{6}$.

\smallskip

\end{itemize}


\item   \begin{enumerate}

\item  If $\Delta t < 0$, then $\sqrt{\Delta t}$ is not a real number.  Hence, $g'(0) = \ds{\lim_{\Delta t \rightarrow 0} \dfrac{g(\Delta t) - g(0)}{\Delta t}}$ does not exist.

\item  $g_{+}'(0) =\ds{ \lim_{\Delta t \rightarrow 0^{+}} (\Delta t)^{\frac{1}{2}}   =  0}$

\smallskip

\item  $y = g_{+}'(0) (x - 0) + g(0) =  (0) (x-0) + 0$ so $y = 0$.  

\smallskip

This line is a tangent line to the graph of $y = t \sqrt{t}$ at $(0,0)$ for $t \geq 0$.

\smallskip

\item  $g'(t) =\ds{ \lim_{\Delta t \rightarrow 0}\dfrac{3t^2+3t\Delta t+(\Delta t)^2}{(t+\Delta t)^{3/2} + t^{3/2}} = \dfrac{3t^2}{2 t^{3/2}} = \dfrac{3}{2} \, t^{1/2}}$ provided $t > 0$.


\end{enumerate}


\setcounter{HW}{\value{enumi}}
\end{enumerate}

\begin{enumerate}
\setcounter{enumi}{\value{HW}}

\item  \begin{enumerate} \item  $g'(t) = \ds{ \lim_{\Delta t \rightarrow 0} \dfrac{a}{\sqrt{at+a\Delta t+b} + \sqrt{at+b}} = \dfrac{a}{2 \sqrt{at+b}} }$.  

\smallskip

\item  We are told $a \neq 0$.  In order for the square roots to be happy, we assume $at + b > 0$.  Hence,   $t >  - \frac{b}{a}$ if $a>0$ and $t < -  \frac{b}{a}$ if $a<0$. 

\end{enumerate}

\setcounter{HW}{\value{enumi}}
\end{enumerate}


\begin{enumerate}
\setcounter{enumi}{\value{HW}}


\item Let  $g(t) = \sqrt[3]{t}$.  

\begin{enumerate}

\item $g'(0) = \ds{ \lim_{\Delta t \rightarrow 0} \dfrac{1}{(\Delta t)^{2/3}}   =  \infty}$

\smallskip

        
\item  The graph of $y = g(t)$ near $(0,0$) is a vertical line.\footnote{We say the graph of $g$ has a  \index{vertical tangent}\index{tangent line ! vertical}\textbf{vertical tangent line} at $t=0$.  This is the more formal way to describe all of the `unusual steepness' we saw back in Chapter \ref{RootRadicalPowerFunctions}.}  Since $g$ is increasing through $(0,0)$, the `slope' of this vertical line could be seen as $+ \infty$. 

\smallskip

\item  Find and simplify  $g'(t) = \ds{ \lim_{\Delta t \rightarrow 0} \dfrac{1}{(t+\Delta t)^{2/3} + (t+\Delta t)^{1/3} t^{1/3} + t^{2/3}} = \dfrac{1}{3 t^{2/3}} }$, $t \neq 0$.

\end{enumerate}

\setcounter{HW}{\value{enumi}}
\end{enumerate}

